# Mon Jun 11 2012

## Review 

\[ d = rt \]

\[ f(b) - f(a) = (b - a) f'\]


### Tayer expansion of \[f\] about \[a\]
\[ f(b) = \sum\limits_{k = 0}^\infty  {\frac{{{f^k}a}}{{k!}}} {\left( {b - a} \right)^k}\]

let \[b = x, a= 0\]

\[ f(x) = \sum\limits_{k = 0}^\infty {\frac{ f^k(o)}{ k!}} x^k\]


### Ex1

\[f(x) = e^x\]

\[f(0) = 1 \]

\[ e^x = \sum\limits_{k = 0}^\infty {\frac{ x^k}{ k!}\]


### Ex2

\[f(x) = (1 +x)^n\]

\[f^k (x) = n(n - 1)(n - 2) \cdots (n - k + 1)(1 + x)^{n - k}\]

\[(1+ x)^n = \sum\limits_{k = 0}^\infty {\frac{ n(n- 1) \cdots (n - k + 1)}{ k!} x^k \], if it converges. 